refactor to use add_mem_var and add_type_var and start fix of adding these vars
previously, the substitution lemmas only had to touch fc_kind_ctx and fc_type_vars. We noticed early on that when adding in a rep or a
size, the kinds in fc_type_vars had to be upshifted, which forced the creation of add_rep_var and add_size_var. However, we forgot that
labels and return contexts also had to upshifted. This is what unpacked existential tried to do, but used up_X stuff instead ren_X, and
then also "double dipped". So, what this is currently doing is making sure that the add_X_var things upshift all occurences of necessary
variables. Doing this changed caused no changes anywhere (understandably since the lemmas never had to deal with labels and return, but
now that I'm doing unpacked which will need them).

unpacked_existential is still not quite correct - it's still trying to use subst_function_ctx, but it should just be F0 := add_X_var F.
Only reason that's not in is because I ran out of time and didn't want to deal with fixing compat_unpack.

theories/kinding_subst.v
@@ -20,7 +20,7 @@ Proof.
 Qed.
 
 Lemma has_kind_var_wk_ty F n κ κv :
-  has_kind (F <| fc_type_vars ::= cons κv |>) (VarT (S n)) κ ↔ has_kind F (VarT n) κ.
+  has_kind (add_type_var F κv) (VarT (S n)) κ ↔ has_kind F (VarT n) κ.
 Proof.
   split; intros Hk.
   - inversion Hk; subst.
@@ -39,14 +39,14 @@ Definition fc_ren (ξr ξs ξt : nat → nat) (F F' : function_ctx) : Prop :=
 Lemma fc_ren_cons ξr ξs ξt F F' κ :
   fc_ren ξr ξs ξt F F' →
   fc_ren ξr ξs (unscoped.up_ren ξt)
-    (F <| fc_type_vars ::= cons κ |>) (F' <| fc_type_vars ::= cons (ren_kind ξr ξs κ) |>).
+    (add_type_var F κ) (add_type_var F' (ren_kind ξr ξs κ)).
 Proof.
   intros HF [|t]; cbn; [done|apply HF].
 Qed.
 
 Lemma fc_ren_mem ξr ξs ξt F F' :
   fc_ren ξr ξs ξt F F' →
-  fc_ren ξr ξs ξt (F <| fc_kind_ctx ::= set kc_mem_vars S |>) (F' <| fc_kind_ctx ::= set kc_mem_vars S |>).
+  fc_ren ξr ξs ξt (add_mem_var F) (add_mem_var F').
 Proof.
   intros HF t; cbn; apply HF.
 Qed.
@@ -215,7 +215,7 @@ Definition ctx_ren (ξm ξr ξs ξt : nat -> nat) (F F' : function_ctx) : Prop :
 Lemma ctx_ren_cons ξm ξr ξs ξt F F' κ :
   ctx_ren ξm ξr ξs ξt F F' ->
   ctx_ren ξm ξr ξs (unscoped.up_ren ξt)
-    (F <| fc_type_vars ::= cons κ |>) (F' <| fc_type_vars ::= cons (ren_kind ξr ξs κ) |>).
+    (add_type_var F κ) (add_type_var F' (ren_kind ξr ξs κ)).
 Proof.
   intros [H1 H2]; split; [by apply fc_ren_cons|].
   by rewrite !fc_kind_ctx_ty_update.
@@ -224,7 +224,7 @@ Qed.
 Lemma ctx_ren_mem ξm ξr ξs ξt F F' :
   ctx_ren ξm ξr ξs ξt F F' ->
   ctx_ren (unscoped.up_ren ξm) ξr ξs ξt
-    (F <| fc_kind_ctx ::= set kc_mem_vars S |>) (F' <| fc_kind_ctx ::= set kc_mem_vars S |>).
+    (add_mem_var F) (add_mem_var F').
 Proof.
   intros [H1 H2]; split; [by apply fc_ren_mem|].
   destruct F, F'; cbn in *; by apply kc_ren_mem.
@@ -388,7 +388,7 @@ Definition ctx_str (ξt : nat -> nat) (F F' : function_ctx) : Prop :=
 Lemma ctx_str_cons ξt F F' κ :
   ctx_str ξt F F' ->
   ctx_str (unscoped.up_ren ξt)
-    (F <| fc_type_vars ::= cons κ |>) (F' <| fc_type_vars ::= cons κ |>).
+    (add_type_var F κ) (add_type_var F' κ).
 Proof.
   intros [Hk Hl]; split; [by rewrite !fc_kind_ctx_ty_update|].
   intros [|t]; unfold unscoped.up_ren, unscoped.scons, core.funcomp;
@@ -397,8 +397,8 @@ Qed.
 
 Lemma ctx_str_mem ξt F F' :
   ctx_str ξt F F' ->
-  ctx_str ξt (F <| fc_kind_ctx ::= set kc_mem_vars S |>)
-             (F' <| fc_kind_ctx ::= set kc_mem_vars S |>).
+  ctx_str ξt (add_mem_var F)
+             (add_mem_var F').
 Proof.
   intros [Hk Hl]; split.
   - destruct F, F'; cbn in *; by rewrite Hk.
@@ -567,14 +567,14 @@ Proof.
     inversion H; subst.
     eapply KRec; last done.
     + by rewrite <- (proj1 Hctx).
-    + eapply (IH ξm ξr ξs (unscoped.up_ren ξt) _ (F' <| fc_type_vars ::= cons κ |>));
+    + eapply (IH ξm ξr ξs (unscoped.up_ren ξt) _ (add_type_var F' κ));
         eauto using ctx_str_cons.
   - intros κ0 t IH ξm ξr ξs ξt F F' κ Hm Hr Hs Hctx H.
     cbn [ren_type] in H; rewrite (ren_kind_id ξr ξs κ0 Hr Hs) in H.
     inversion H; subst.
     apply KExistsMem; [by rewrite -(proj1 Hctx)|].
     eapply (IH (unscoped.up_ren ξm) ξr ξs ξt _
-              (F' <| fc_kind_ctx ::= set kc_mem_vars S |>));
+              (add_mem_var F'));
       eauto using ctx_str_mem, pw_id_up.
   - intros κ0 t IH ξm ξr ξs ξt F F' κ Hm Hr Hs Hctx H.
     cbn [ren_type] in H; rewrite (ren_kind_id ξr ξs κ0 Hr Hs) in H.
@@ -593,7 +593,7 @@ Proof.
     rewrite (ren_kind_id ξr ξs κ1 Hr Hs) (ren_kind_id ξr ξs κ2 Hr Hs) in H.
     inversion H; subst.
     apply KExistsType; [by rewrite -(proj1 Hctx)|by rewrite -(proj1 Hctx)|].
-    eapply (IH ξm ξr ξs (unscoped.up_ren ξt) _ (F' <| fc_type_vars ::= cons κ2 |>));
+    eapply (IH ξm ξr ξs (unscoped.up_ren ξt) _ (add_type_var F' κ2));
       eauto using ctx_str_cons.
   - intros τs1 τs2 IH1 IH2 ξm ξr ξs ξt F F' Hm Hr Hs Hctx H.
     cbn [ren_inner_function_type] in H.
@@ -608,7 +608,7 @@ Proof.
     rewrite (ren_kind_id ξr ξs κ0 Hr Hs) in H.
     inversion H; subst.
     apply KForallType; [by rewrite -(proj1 Hctx)|].
-    eapply (IH ξm ξr ξs (unscoped.up_ren ξt) _ (F' <| fc_type_vars ::= cons κ0 |>));
+    eapply (IH ξm ξr ξs (unscoped.up_ren ξt) _ (add_type_var F' κ0));
       eauto using ctx_str_cons.
   - intros ft IH ξm ξr ξs ξt F F' Hm Hr Hs Hctx H.
     cbn [ren_function_type] in H.
@@ -620,7 +620,7 @@ Proof.
     inversion H; subst.
     apply KForallMem.
     eapply (IH (unscoped.up_ren ξm) ξr ξs ξt _
-              (F' <| fc_kind_ctx ::= set kc_mem_vars S |>));
+              (add_mem_var F'));
       eauto using ctx_str_mem, pw_id_up.
   - intros ft IH ξm ξr ξs ξt F F' Hm Hr Hs Hctx H.
     cbn [ren_function_type] in H.
@@ -640,7 +640,7 @@ Lemma kc_ren_refl K : kc_ren (@id nat) (@id nat) (@id nat) K K.
 Proof. unfold kc_ren; split; [|split]; intros n; reflexivity. Qed.
 
 Lemma ctx_ren_wk F κv :
-  ctx_ren (@id nat) (@id nat) (@id nat) S F (F <| fc_type_vars ::= cons κv |>).
+  ctx_ren (@id nat) (@id nat) (@id nat) S F (add_type_var F κv).
 Proof.
   split; [|by rewrite fc_kind_ctx_ty_update; apply kc_ren_refl].
   intros t; rewrite fc_type_vars_get_upd.
@@ -649,20 +649,20 @@ Proof.
   by rewrite (ren_kind_id (@id nat) (@id nat) κ0 pw_id_id pw_id_id).
 Qed.
 
-Lemma ctx_str_wk F κv : ctx_str S F (F <| fc_type_vars ::= cons κv |>).
+Lemma ctx_str_wk F κv : ctx_str S F (add_type_var F κv).
 Proof.
   split; [by rewrite fc_kind_ctx_ty_update|].
   intros t; by rewrite fc_type_vars_get_upd.
 Qed.
 
 Lemma has_kind_wk_ty F τ κ κv :
-  has_kind F τ κ ↔ has_kind (F <| fc_type_vars ::= cons κv |>) (ren_type id id id S τ) κ.
+  has_kind F τ κ ↔ has_kind (add_type_var F κv) (ren_type id id id S τ) κ.
 Proof.
   split; intros Hk.
   - rewrite -(ren_kind_id (@id nat) (@id nat) κ pw_id_id pw_id_id).
     by apply (has_kind_ren _ _ _ Hk), ctx_ren_wk.
   - eapply (proj1 has_kind_ren_inv τ (@id nat) (@id nat) (@id nat) S F
-                  (F <| fc_type_vars ::= cons κv |>));
+                  (add_type_var F κv));
       eauto using pw_id_id, ctx_str_wk.
 Qed.
 
@@ -846,7 +846,7 @@ Proof.
     inversion Hk; subst; inversion Hr; subst; f_equal; try done;
       by eapply IH; eauto.
   - intros ft IH F ϕ' Hk Hr.
-    inversion Hk; subst; inversion Hr; subst; f_equal; try done;
+    inversion Hk; subst; inversion Hr; subst; f_equal; try done.
       by eapply IH; eauto.
   - intros ft IH F ϕ' Hk Hr.
     inversion Hk; subst; inversion Hr; subst; f_equal; try done;
@@ -922,7 +922,7 @@ Qed.
 
 Lemma ctx_ren_wk_mem F :
   ctx_ren unscoped.shift (@id nat) (@id nat) (@id nat) F
-    (F <| fc_kind_ctx ::= set kc_mem_vars S |>).
+    (add_mem_var F).
 Proof.
   split.
   - intros t; destruct F as [? ? ? ? tvs]; cbn.
@@ -1148,7 +1148,7 @@ Lemma ctx_rel_cons R σm σr σs σt F F' κ0 :
   kind_rel_ok R ->
   ctx_rel R σm σr σs σt F F' ->
   ctx_rel R (up_type_memory σm) (up_type_representation σr) (up_type_size σs) (up_type_type σt)
-    (F <| fc_type_vars ::= cons κ0 |>) (F' <| fc_type_vars ::= cons (subst_kind σr σs κ0) |>).
+    (add_type_var F κ0) (add_type_var F' (subst_kind σr σs κ0)).
 Proof.
   intros [Hrefl _] [Hkc Hv]; split; [rewrite !fc_kind_ctx_ty_update; by apply kc_subst_type|].
   intros [|t] κ Hk.
@@ -1169,7 +1169,7 @@ Lemma ctx_rel_mem R σm σr σs σt F F' :
   ctx_rel R σm σr σs σt F F' ->
   ctx_rel R (up_memory_memory σm) (up_memory_representation σr) (up_memory_size σs)
     (up_memory_type σt)
-    (F <| fc_kind_ctx ::= set kc_mem_vars S |>) (F' <| fc_kind_ctx ::= set kc_mem_vars S |>).
+    (add_mem_var F) (add_mem_var F').
 Proof.
   intros [Hkc Hv]; split; [destruct F, F'; cbn in *; by apply kc_subst_mem|].
   intros t κ Hk.
@@ -1302,8 +1302,8 @@ Proof.
     eapply KRec.
     + by eapply kind_ok_subst; [apply Hctx|].
     + eapply (IH (up_type_memory σm) (up_type_representation σr) (up_type_size σs)
-                (up_type_type σt) (F <| fc_type_vars ::= cons κ |>)
-                (F' <| fc_type_vars ::= cons (subst_kind σr σs κ) |>));
+                (up_type_type σt) (add_type_var F κ)
+                (add_type_var F' (subst_kind σr σs κ)));
         eauto using sub_id_up_type_memory, ctx_rel_cons, kind_rel_ok_eq.
     + rewrite subst_kind_up_type; by apply subkind_of_subst.
   - intros κ0 t IH σm σr σs σt F F' κ Hm Hctx Hk.
@@ -1311,8 +1311,8 @@ Proof.
     apply KExistsMem; [by eapply kind_ok_subst; [apply Hctx|]|].
     rewrite -subst_kind_up_mem.
     eapply (IH (up_memory_memory σm) (up_memory_representation σr) (up_memory_size σs)
-              (up_memory_type σt) (F <| fc_kind_ctx ::= set kc_mem_vars S |>)
-              (F' <| fc_kind_ctx ::= set kc_mem_vars S |>));
+              (up_memory_type σt) (add_mem_var F)
+              (add_mem_var F'));
       eauto using sub_id_up_memory_memory, ctx_rel_mem.
   - intros κ0 t IH σm σr σs σt F F' κ Hm Hctx Hk.
     inversion Hk; subst; cbn.
@@ -1334,8 +1334,8 @@ Proof.
     apply KExistsType; [by eapply kind_ok_subst; [apply Hctx|]|by eapply kind_ok_subst; [apply Hctx|]|].
     rewrite -(subst_kind_up_type σr σs κ).
     eapply (IH (up_type_memory σm) (up_type_representation σr) (up_type_size σs)
-              (up_type_type σt) (F <| fc_type_vars ::= cons κ2 |>)
-              (F' <| fc_type_vars ::= cons (subst_kind σr σs κ2) |>));
+              (up_type_type σt) (add_type_var F κ2)
+              (add_type_var F' (subst_kind σr σs κ2)));
       eauto using sub_id_up_type_memory, ctx_rel_cons, kind_rel_ok_eq.
   - intros τs1 τs2 IH1 IH2 σm σr σs σt F F' Hm Hctx Hk.
     inversion Hk; subst; cbn.
@@ -1350,8 +1350,8 @@ Proof.
     inversion Hk; subst; cbn.
     apply KForallType; [by eapply kind_ok_subst; [apply Hctx|]|].
     eapply (IH (up_type_memory σm) (up_type_representation σr) (up_type_size σs)
-              (up_type_type σt) (F <| fc_type_vars ::= cons κ0 |>)
-              (F' <| fc_type_vars ::= cons (subst_kind σr σs κ0) |>));
+              (up_type_type σt) (add_type_var F κ0)
+              (add_type_var F' (subst_kind σr σs κ0)));
       eauto using sub_id_up_type_memory, ctx_rel_cons, kind_rel_ok_eq.
   - intros ft IH σm σr σs σt F F' Hm Hctx Hk.
     inversion Hk; subst; cbn.
@@ -1360,8 +1360,8 @@ Proof.
     inversion Hk; subst; cbn.
     apply KForallMem.
     eapply (IH (up_memory_memory σm) (up_memory_representation σr) (up_memory_size σs)
-              (up_memory_type σt) (F <| fc_kind_ctx ::= set kc_mem_vars S |>)
-              (F' <| fc_kind_ctx ::= set kc_mem_vars S |>));
+              (up_memory_type σt) (add_mem_var F)
+              (add_mem_var F'));
       eauto using sub_id_up_memory_memory, ctx_rel_mem.
   - intros ft IH σm σr σs σt F F' Hm Hctx Hk.
     inversion Hk; subst; cbn.
@@ -1416,7 +1416,7 @@ Qed.
 
 Lemma ctx_subst_scons F τv κv :
   has_kind F τv κv ->
-  ctx_subst (unscoped.scons τv VarT) (F <| fc_type_vars ::= cons κv |>) F.
+  ctx_subst (unscoped.scons τv VarT) (add_type_var F κv) F.
 Proof.
   intros Hv; split; [by rewrite fc_kind_ctx_ty_update|].
   intros [|t] κ Hk.
@@ -1429,7 +1429,7 @@ Qed.
 Lemma has_kind_env_to_has_kind_subst τ : ∀ F τv κv κ τ',
   refreshed_kinds F (subst_type VarM VarR VarS (unscoped.scons τv VarT) τ) τ' →
   has_kind F τv κv →
-  has_kind (F <| fc_type_vars ::= cons κv |>) τ κ →
+  has_kind (add_type_var F κv) τ κ →
   has_kind F τ' κ.
 Proof.
   intros F τv κv κ τ' Hrefresh Hv Hkind.
@@ -1442,7 +1442,7 @@ Qed.
 Lemma has_kinds_env_to_has_kinds_subst τs : ∀ F τv κv κs τs',
   Forall2 (refreshed_kinds F) (map (subst_type VarM VarR VarS (unscoped.scons τv VarT)) τs) τs' →
   has_kind F τv κv →
-  Forall2 (has_kind (F <| fc_type_vars ::= cons κv |>)) τs κs →
+  Forall2 (has_kind (add_type_var F κv)) τs κs →
   Forall2 (has_kind F) τs' κs.
 Proof.
   induction τs as [|τ τs IH]; intros F τv κv κs τs' Hrefresh Hv Hkind; cbn in Hrefresh.
@@ -1458,7 +1458,7 @@ Lemma needs_name_fwd ϕ F τ κ ϕ' :
   has_kind F τ κ →
   refreshed_kinds_ift F
     (subst_inner_function_type VarM VarR VarS (unscoped.scons τ VarT) ϕ) ϕ' →
-  has_kind_ift (F <| fc_type_vars ::= cons κ |>) ϕ →
+  has_kind_ift (add_type_var F κ) ϕ →
   has_kind_ift F ϕ'.
 Proof.
   intros Ht Hrf Hk.
@@ -1580,10 +1580,10 @@ Fixpoint refresh_kinds (F : function_ctx) (τ : type) : type :=
       SerT κ τ'
   | PlugT _ ρ => PlugT (VALTYPE ρ NoRefs) ρ
   | SpanT _ σ => SpanT (MEMTYPE σ NoRefs) σ
-  | RecT κ τ => RecT κ (refresh_kinds (F <| fc_type_vars ::= cons κ |>) τ)
+  | RecT κ τ => RecT κ (refresh_kinds (add_type_var F κ) τ)
   | ExistsMemT _ τ =>
-      let τ' := refresh_kinds (F <| fc_kind_ctx ::= set kc_mem_vars S |>) τ in
-      let κ := kind_of_node ((F <| fc_kind_ctx ::= set kc_mem_vars S |>)) τ' in
+      let τ' := refresh_kinds (add_mem_var F) τ in
+      let κ := kind_of_node ((add_mem_var F)) τ' in
       ExistsMemT κ τ'
   | ExistsRepT _ τ =>
       let τ' := refresh_kinds (add_rep_var F) τ in
@@ -1592,19 +1592,19 @@ Fixpoint refresh_kinds (F : function_ctx) (τ : type) : type :=
       let τ' := refresh_kinds (add_size_var F) τ in
       ExistsSizeT (unshift_size_kind (kind_of_node (add_size_var F) τ')) τ'
   | ExistsTypeT _ κ0 τ =>
-      let τ' := refresh_kinds (F <| fc_type_vars ::= cons κ0 |>) τ in
-      let κ := kind_of_node ((F <| fc_type_vars ::= cons κ0 |>)) τ' in
+      let τ' := refresh_kinds (add_type_var F κ0) τ in
+      let κ := kind_of_node ((add_type_var F κ0)) τ' in
       ExistsTypeT κ κ0 τ'
   end
 with refresh_kinds_ift (F : function_ctx) (ϕ : inner_function_type) : inner_function_type :=
        match ϕ with
        | MonoFunT τs1 τs2 => MonoFunT (map (refresh_kinds F) τs1) (map (refresh_kinds F) τs2)
-       | ForallTypeT κ ϕ => ForallTypeT κ (refresh_kinds_ift (F <| fc_type_vars ::= cons κ |>) ϕ)
+       | ForallTypeT κ ϕ => ForallTypeT κ (refresh_kinds_ift (add_type_var F κ) ϕ)
        end
 with refresh_kinds_ft (F : function_ctx) (ϕ : Core.function_type) : Core.function_type :=
        match ϕ with
        | InnerFunT ϕ => InnerFunT (refresh_kinds_ift F ϕ)
-       | ForallMemT ϕ => ForallMemT (refresh_kinds_ft (F <| fc_kind_ctx ::= set kc_mem_vars S |>) ϕ)
+       | ForallMemT ϕ => ForallMemT (refresh_kinds_ft (add_mem_var F) ϕ)
        | ForallRepT ϕ => ForallRepT (refresh_kinds_ft (add_rep_var F) ϕ)
        | ForallSizeT ϕ => ForallSizeT (refresh_kinds_ft (add_size_var F) ϕ)
        end.
@@ -1882,7 +1882,7 @@ Proof.
 Qed.
 
 Lemma refresh_kinds_up_shift_type F κ τ :
-  refresh_kinds (F <| fc_type_vars ::= cons κ |>)
+  refresh_kinds (add_type_var F κ)
     (ren_type unscoped.id unscoped.id unscoped.id unscoped.shift τ) =
   ren_type unscoped.id unscoped.id unscoped.id unscoped.shift (refresh_kinds F τ).
 Proof.
@@ -1892,7 +1892,7 @@ Proof.
 Qed.
 
 Lemma refresh_kinds_up_shift_mem F τ :
-  refresh_kinds (F <| fc_kind_ctx ::= set kc_mem_vars S |>)
+  refresh_kinds (add_mem_var F)
     (ren_type unscoped.shift unscoped.id unscoped.id unscoped.id τ) =
   ren_type unscoped.shift unscoped.id unscoped.id unscoped.id (refresh_kinds F τ).
 Proof.
@@ -2247,7 +2247,7 @@ Proof.
     apply KSpan; by eapply size_ok_subst; [apply Hctx|].
   - intros κ0 t IH σm σr σs σt F F' κ Hctx Hk.
     inversion Hk; subst; cbn.
-    match goal with H : has_kind (F <| fc_type_vars ::= cons κ |>) t _ |- _ =>
+    match goal with H : has_kind (add_type_var F κ) t _ |- _ =>
       destruct (IH _ _ _ _ _ _ _ (ctx_rel_cons _ _ _ _ _ _ _ κ kind_rel_ok_subkind Hctx) H)
         as (κ' & Hsub & Hk')
     end.
@@ -2312,7 +2312,7 @@ Proof.
   - intros κ0 ft IH σm σr σs σt F F' Hctx Hk.
     inversion Hk; subst; cbn.
     apply KForallType; [by eapply kind_ok_subst; [apply Hctx|]|].
-    eapply (IH _ _ _ _ (F <| fc_type_vars ::= cons κ0 |>) _);
+    eapply (IH _ _ _ _ (add_type_var F κ0) _);
       [by apply ctx_rel_cons; [exact kind_rel_ok_subkind|exact Hctx]|done].
   - intros ft IH σm σr σs σt F F' Hctx Hk.
     inversion Hk; subst; cbn.
@@ -2320,7 +2320,7 @@ Proof.
   - intros ft IH σm σr σs σt F F' Hctx Hk.
     inversion Hk; subst; cbn.
     apply KForallMem.
-    eapply (IH _ _ _ _ (F <| fc_kind_ctx ::= set kc_mem_vars S |>) _);
+    eapply (IH _ _ _ _ (add_mem_var F) _);
       [by apply ctx_rel_mem|done].
   - intros ft IH σm σr σs σt F F' Hctx Hk.
     inversion Hk; subst; cbn.
@@ -2337,7 +2337,7 @@ Qed.
 Lemma ctx_rel_inst_type F τ κ κ' :
   has_kind F τ κ' -> subkind_of κ' κ ->
   ctx_rel subkind_of VarM VarR VarS (unscoped.scons τ VarT)
-    (F <| fc_type_vars ::= cons κ |>) F.
+    (add_type_var F κ) F.
 Proof.
   intros Ht Hsub; split.
   - rewrite fc_kind_ctx_ty_update; split; [|split]; intros n Hn; by constructor.
@@ -2353,7 +2353,7 @@ Qed.
 Lemma ctx_rel_inst_mem F μ :
   mem_ok (fc_kind_ctx F) μ ->
   ctx_rel subkind_of (unscoped.scons μ VarM) VarR VarS VarT
-    (F <| fc_kind_ctx ::= set kc_mem_vars S |>) F.
+    (add_mem_var F) F.
 Proof.
   intros Hμ; split.
   - split; [|split].
@@ -2462,7 +2462,7 @@ Definition ctx_le (F F' : function_ctx) : Prop :=
   forall t κ, fc_type_vars F !! t = Some κ -> fc_type_vars F' !! t = Some κ.
 
 Lemma ctx_le_cons F F' κ :
-  ctx_le F F' -> ctx_le (F <| fc_type_vars ::= cons κ |>) (F' <| fc_type_vars ::= cons κ |>).
+  ctx_le F F' -> ctx_le (add_type_var F κ) (add_type_var F' κ).
 Proof.
   intros [Hkc Hv]; split; [by rewrite !fc_kind_ctx_ty_update|].
   intros [|t] κ0; rewrite !fc_type_vars_get_upd; [done|by apply Hv].
@@ -2470,7 +2470,7 @@ Qed.
 
 Lemma ctx_le_mem F F' :
   ctx_le F F' ->
-  ctx_le (F <| fc_kind_ctx ::= set kc_mem_vars S |>) (F' <| fc_kind_ctx ::= set kc_mem_vars S |>).
+  ctx_le (add_mem_var F) (add_mem_var F').
 Proof.
   intros [(Hm & Hr & Hs) Hv]; split; [|by rewrite !fc_type_vars_kc_update].
   destruct F as [? ? ? [] ?], F' as [? ? ? [] ?]; unfold kc_le in *; cbn in *; split; [|split]; lia.
